core/Coqlib.v
@@ -1,4 +1,20 @@
 Require Export Coq.Lists.List.
+Require Export Coq.ssr.ssrbool.
 Export ListNotations.
 
 Notation "~~" := negb.
+
+Ltac inv H := inversion H; subst; clear H.
+Ltac pinv P :=
+  lazymatch goal with
+  | H : context [P] |- _ => inv H
+  (* | H : P |- _ => inv H
+  | H : P _ |- _ => inv H
+  | H : P _ _ |- _ => inv H
+  | H : P _ _ _ |- _ => inv H
+  | H : P _ _ _ _ |- _ => inv H
+  | H : P _ _ _ _ _ |- _ => inv H
+  | H : P _ _ _ _ _ _ |- _ => inv H
+  | H : P _ _ _ _ _ _ _ |- _ => inv H
+  | H : P _ _ _ _ _ _ _ _ |- _ => inv H *)
+  end.
